fix mk_runtime exp and mont

code/bignum/Hacl.Bignum.Montgomery.fst
@@ -237,3 +237,9 @@ let mk_runtime_mont_uint64 (len: BN.meta_len U64) : mont U64 = {
   mul = mul_runtime_u64 len;
   sqr = sqr_runtime_u64 len;
 }
+
+
+let mk_runtime_mont (#t:limb_t) (len:BN.meta_len t) : mont t =
+  match t with
+  | U32 -> mk_runtime_mont_uint32 len
+  | U64 -> mk_runtime_mont_uint64 len
